<?xml version="1.0"?>
<rdf:RDF xmlns="https://digital-humanities.at/schema"
     xml:base="https://digital-humanities.at/schema"
     xmlns:dct="http://purl.org/dc/terms/"
     xmlns:rdf="http://www.w3.org/1999/02/22-rdf-syntax-ns#"
     xmlns:owl="http://www.w3.org/2002/07/owl#"
     xmlns:xml="http://www.w3.org/XML/1998/namespace"
     xmlns:xsd="http://www.w3.org/2001/XMLSchema#"
     xmlns:skos="http://www.w3.org/2004/02/skos/core#"
     xmlns:rdfs="http://www.w3.org/2000/01/rdf-schema#"
     xmlns:acdh="https://vocabs.acdh.oeaw.ac.at/schema#"
     xmlns:foaf="http://xmlns.com/foaf/spec/#"
 
    xmlns:dc="http://purl.org/dc/elements/1.1/">
    <owl:Ontology rdf:about="https://digital-humanities.at/schema">
<rdfs:label>DHA Ontology</rdfs:label>
    
        <rdfs:comment xml:lang="en">Dies ist die gemeinsame Ontologie für Digital Humanities Austria. Sie dient der Beschreibung von digitalen Objekten im Kontext der DH-Forschung.</rdfs:comment>
<rdfs:comment>In den Definitionen der Eigenschaften, meint &quot;Ressource A&quot; das Subject und &quot;Ressource B&quot; das Objekt.
When Definitionen aus anderen Schemata (z. B. DataCite) wiederverwendet werden, wird die Referenz in Klammern angegeben: (DataCite: ContactPerson). When die ursprüngliche Definition leicht angepasst wurde, ist die Referenz mit &quot;cf.&quot; markiert.</rdfs:comment>
        <rdfs:comment xml:lang="en">This is the ontology for Digital Humanities Austria. It serves the description of digital objects in the context of DH-research.</rdfs:comment>
<rdfs:comment>In definitions of properties, &quot;resource A&quot; refers to the subject resource of the property and &quot;resource B&quot; to the object resource.
When reusing definitions from other vocabularies (esp. DataCite), the reference is given in brackets: (DataCite: ContactPerson). When the source definition was changed slightly the reference is marked with &quot;cf.&quot;</rdfs:comment>        
        <owl:versionInfo xml:lang="de">2019-04-05 - Erste Fassung *native"-Ansatz (Klassen und properties im eigenen Namespace) - basierend auf dem KONDE Workshop, Wien 2019-03-12/13; ausgehend von dem acdh-schema.owl [https://digital-humanities.at/schema]</owl:versionInfo>
        
    </owl:Ontology>


    <!-- 
    ///////////////////////////////////////////////////////////////////////////////////////
    //
    // Object Properties
    //
    ///////////////////////////////////////////////////////////////////////////////////////
     -->

    

    <!-- http://purl.org/dc/elements/1.1/contributor -->

    <owl:ObjectProperty rdf:about="http://purl.org/dc/elements/1.1/contributor">
        <owl:equivalentProperty rdf:resource="https://digital-humanities.at/schema#hasContributor"/>
    </owl:ObjectProperty>
    

    <!-- https://digital-humanities.at/schema#hasContributor -->

    <owl:ObjectProperty rdf:about="https://digital-humanities.at/schema#hasContributor">
        <rdfs:subPropertyOf rdf:resource="http://www.w3.org/2002/07/owl#topObjectProperty"/>
        <owl:inverseOf rdf:resource="https://digital-humanities.at/schema#isContributorOf"/>
        <rdfs:domain rdf:resource="https://digital-humanities.at/schema#Main"/>
        <rdfs:range rdf:resource="https://digital-humanities.at/schema#Agent"/>
        <rdfs:comment xml:lang="en">Agent (person, group, organisation) (B) who was actively involved in creating/curating/editing a Resource, a Collection or in a Project (A). Any person or institution making a significant contribution to the development and/or maintenance of the resource, but whose contribution does not “fit” to another already defined role. (cf. DataCite: Other)
This is a generic property. Use one of the more specific sub-properties where possible.</rdfs:comment>
        <rdfs:label xml:lang="en">has contributor</rdfs:label>
        <skos:altLabel xml:lang="en">Contributor(s)</skos:altLabel>
        <skos:altLabel xml:lang="de">Mitarbeiter oder Beitragende(r)</skos:altLabel>
        <acdh:ordering rdf:datatype="http://www.w3.org/2001/XMLSchema#integer">60</acdh:ordering>
    </owl:ObjectProperty>
   
   
    <!-- 
    ///////////////////////////////////////////////////////////////////////////////////////
    //
    // Datatype Properties
    //
    ///////////////////////////////////////////////////////////////////////////////////////
     -->



    <owl:DatatypeProperty rdf:about="https://digital-humanities.at/schema#hasIdentifier">
        <rdfs:subPropertyOf rdf:resource="http://www.w3.org/2002/07/owl#topDataProperty"/>
        <rdfs:domain rdf:resource="https://digital-humanities.at/schema#Main"/>
        <rdfs:range rdf:resource="http://www.w3.org/2001/XMLSchema#anyURI"/>
        <rdfs:comment xml:lang="en">Unique identifier given by ACDH and used in ACDH systems, as well as identifiers with a stable URL or URI assigned by other parties, e. g. a DOI, a geonames ID or an URN.
Input as URI.
Handles belong into acdh:hasPID and all other identifiers without URL or URI, like local assigned ones, project numbers or inventory numbers into acdh:hasNonLinkedIdentifier.</rdfs:comment>
        <rdfs:label xml:lang="en">has identifier</rdfs:label>
        <skos:altLabel xml:lang="en">Identifier(s)</skos:altLabel>
        <skos:altLabel xml:lang="de">Identifikator(en)</skos:altLabel>        
    </owl:DatatypeProperty>
    


    <!-- 
    ///////////////////////////////////////////////////////////////////////////////////////
    //
    // Classes
    //
    ///////////////////////////////////////////////////////////////////////////////////////
     -->
    
	
    <!-- https://vocabs.acdh.oeaw.ac.at/schema#Main -->

    <owl:Class rdf:about="https://vocabs.acdh.oeaw.ac.at/schema#Main"/>
    



    <!-- https://digital-humanities.at/schema#RepoObject -->

    <owl:Class rdf:about="https://digital-humanities.at/schema#RepoObject">
        <rdfs:comment xml:lang="en">Generic entity representing the items in the repository - Collections and Resources, which are modelled as subclasses of Repo Object.</rdfs:comment>
        <rdfs:comment xml:lang="en">Note that other classes, especially Project, are not considered subclasses of Repo Object.</rdfs:comment>
        <rdfs:label>Repo Object</rdfs:label>
    </owl:Class>
   


    <!-- https://digital-humanities.at/schema#Resource -->

    <owl:Class rdf:about="https://digital-humanities.at/schema#Resource">
        
        <rdfs:comment xml:lang="en">Basic entity in the schema containing actual data / content payload; comparable (and mostly equivalent) to files in a file system.</rdfs:comment>
        <rdfs:label xml:lang="en">Resource</rdfs:label>
        <skos:altLabel xml:lang="en">Resource</skos:altLabel>
        <skos:altLabel xml:lang="de">Ressource</skos:altLabel>
    </owl:Class>


    <!-- https://digital-humanities.at/schema#Agent -->

    <owl:Class rdf:about="https://digital-humanities.at/schema#Agent">
        <rdfs:comment xml:lang="en">Entity able to act, in the context of this schema especially be involved in the making, processing, distributing, publishing etc. of a Resource, Collection, Concept or Project.
Note that in contrast to foaf:Agent acdh:Agent can only be a Person or an Organisation (not a software or physical artifact).
The different roles an Agent can assume with respect to a Project, Collection, Resource or Concept are modeled as separate object properties (sub-properties of acdh:contributedTo).</rdfs:comment>
        <rdfs:label xml:lang="en">Agent</rdfs:label>
        <skos:altLabel xml:lang="en">Agent</skos:altLabel>
        <skos:altLabel xml:lang="de">Akteur</skos:altLabel>
		<owl:equivalentClass rdf:resource="http://xmlns.com/foaf/0.1/Agent"/>
    </owl:Class>
    
    
</rdf:RDF>



<!-- Generated by the OWL API (version 4.2.8.20170104-2310) https://github.com/owlcs/owlapi -->

